HMAC_common_defs.v
@@ -1,0 +1,55 @@
+Require Import HMAC_functional_prog.
+Require Import SHA256.
+Require Import ByteBitRelations.
+Require Import Integers.
+Require Import sha_padding_lemmas.
+Require Import Recdef.
+Require Import List.
+Require Import Arith.
+
+Definition Blist := list bool.
+
+Definition concat {A : Type} (l : list (list A)) : list A :=
+  flat_map id l.
+
+(* Replacing splitVector *)
+Definition splitList {A : Type} (n : nat) (l : list A) : (list A * list A) :=
+  (firstn n l, skipn n l).
+
+(* Replacing BVxor *)
+Definition BLxor (xs : Blist) (ys : Blist) :=
+  map (fun p => xorb (fst p) (snd p)) (combine xs ys).
+
+Function hash_blocks_bits (hash_block_bit : Blist -> Blist -> Blist) (r: Blist)
+         (msg: Blist) {measure length msg} : Blist :=
+  match msg with
+  | nil => r
+  | _ => hash_blocks_bits hash_block_bit (hash_block_bit r (firstn 512 msg)) (skipn 512 msg)
+  end.
+Proof. intros.
+ destruct (lt_dec (length msg) 512). 
+ rewrite skipn_length_short. simpl; omega. rewrite <- teq; auto.
+ rewrite skipn_length. simpl; omega. rewrite <- teq; omega.
+Defined.
+
+
+(* TODO use neater definition with conversion functions *)
+(* TODO split out of HMAC_spec_pad *)
+
+Definition c := (SHA256_.DigestLength * 8)%nat.
+Definition p := (32 * 8)%nat.
+
+Definition intsToBits (l : list int) : list bool :=
+  bytesToBits (SHA256.intlist_to_Zlist l).
+
+Definition bitsToInts (l : Blist) : list int :=
+  SHA256.Zlist_to_intlist (bitsToBytes l).
+
+Definition sha_iv : Blist :=
+  intsToBits SHA256.init_registers.
+
+Definition sha_h (regs : Blist) (block : Blist) : Blist :=
+  intsToBits (SHA256.hash_block (bitsToInts regs) (bitsToInts block)).
+
+Definition sha_splitandpad (msg : Blist) : Blist :=
+  bytesToBits (sha_padding_lemmas.pad (bitsToBytes msg)).
